IrisCore/CoreStructures.thy
@@ -1,125 +1,9 @@
 theory CoreStructures
-imports OFEs
+imports COFEs
 begin
 
 section \<open> Core Structures \<close>
 text \<open> This section introduces the concepts of cameras, resource algebras and related structures. \<close>
-subsection \<open>Non-expansive functions\<close>
-text \<open>Non-expansive functions, i.e. equivalence persisting functions from one OFE to another.\<close>
-definition non_expansive :: "('a::ofe \<Rightarrow>'b::ofe) \<Rightarrow> bool" where 
-  "non_expansive ne \<equiv> \<forall>x y n. n_equiv n x y \<longrightarrow> n_equiv n (ne x) (ne y)"
-
-lemma non_expansiveI[intro?]: "\<lbrakk>\<And>n x y. n_equiv n x y \<Longrightarrow> n_equiv n (f x) (f y)\<rbrakk> \<Longrightarrow> non_expansive f"
-  unfolding non_expansive_def by simp
-lemma non_expansiveE[elim]: "non_expansive f \<Longrightarrow> 
-  (\<And>n x y. \<lbrakk>n_equiv n x y; f x=x'; f y=y'\<rbrakk> \<Longrightarrow> n_equiv n x' y')"
-  using non_expansive_def by blast
-
-definition non_expansive2 :: "('a::ofe \<Rightarrow> 'b::ofe \<Rightarrow> 'c::ofe) \<Rightarrow> bool" where
-  "non_expansive2 ne \<equiv> \<forall>x y a b n. n_equiv n x y \<longrightarrow> n_equiv n a b \<longrightarrow> n_equiv n (ne x a) (ne y b)"
-
-lemma non_expansive2I[intro?]: "(\<And>x y a b n. n_equiv n x y \<Longrightarrow> n_equiv n a b \<Longrightarrow> 
-  n_equiv n (f x a) (f y b)) \<Longrightarrow> non_expansive2 f"
-  using non_expansive2_def by blast
-lemma non_expansive2E[elim]: "non_expansive2 f \<Longrightarrow> 
-  (\<And>n x y a b. \<lbrakk>n_equiv n x y; n_equiv n a b; f x a=x'; f y b=y'\<rbrakk> \<Longrightarrow> n_equiv n x' y')"
-  using non_expansive2_def by blast
-
-lemma non_expansive2_ne:"non_expansive2 f \<Longrightarrow> non_expansive (f x)"
-  by (auto simp: non_expansive_def non_expansive2_def ofe_eq_limit)
-
-lemma sprop_ne: "non_expansive (Rep_sprop P)"
-  unfolding non_expansive_def n_equiv_nat_def n_equiv_bool_def by simp
-  
-lemma ne_sprop_weaken: 
-  "\<lbrakk>n_equiv n x y; m\<le>n; non_expansive P; Rep_sprop (P x) n\<rbrakk> \<Longrightarrow> Rep_sprop (P y) m"
-  using Rep_sprop n_equiv_sprop_def non_expansive_def by blast
-
-lemma ne_sprop_weaken2:
-  "\<lbrakk>n_equiv n x y; n_equiv n a b; m\<le>n; non_expansive2 P; Rep_sprop (P x a) n\<rbrakk> \<Longrightarrow> Rep_sprop (P y b) m"
-  using Rep_sprop n_equiv_sprop_def non_expansive2_def by fast
-
-lemma ne_comp: "\<lbrakk>non_expansive f; non_expansive g\<rbrakk> \<Longrightarrow> non_expansive (f \<circ> g)"
-  by (auto simp: non_expansive_def)
-
-lemma discrete_ne: "non_expansive (f::'a::discrete\<Rightarrow>'b::discrete)"
-  by (rule non_expansiveI) (simp add: d_equiv)
-  
-text \<open>The corresponding subtype of non-expansive functions.\<close>
-typedef (overloaded) ('a, 'b) ne = "{f::'a::ofe\<Rightarrow>'b::ofe. non_expansive f}"
-  using sprop_ne[of sTrue] apply simp
-  by (metis non_expansiveI ofe_refl)
-type_notation ne (infix "-n>" 60)
-setup_lifting type_definition_ne
-lemmas [simp] = Rep_ne_inverse Rep_ne_inject
-lemmas [simp, intro!] = Rep_ne[unfolded mem_Collect_eq]
-
-instantiation ne :: (ofe,ofe) ofe begin
-lift_definition n_equiv_ne :: "nat \<Rightarrow> 'a-n>'b \<Rightarrow> 'a-n>'b \<Rightarrow> bool" is
-  "\<lambda>n f g. \<forall>x. n_equiv n (f x) (g x)" .
-lift_definition ofe_eq_ne :: "'a-n>'b \<Rightarrow> 'a-n>'b \<Rightarrow> bool" is
-  "\<lambda>f g. \<forall>x. ofe_eq  (f x) (g x)" .
-instance by (standard; transfer) (auto simp: ofe_refl ofe_sym ofe_limit intro: ofe_trans ofe_mono)
-end
-
-lift_definition ne_chain :: "('a::ofe,'b::ofe) ne chain \<Rightarrow> 'a \<Rightarrow> 'b chain" is
-  "\<lambda>c x n. Rep_ne (c n) x" apply transfer unfolding non_expansive_def by auto
-  
-instantiation ne :: (ofe,cofe) cofe begin
-lift_definition lim_ne :: "('a, 'b) ne chain \<Rightarrow> ('a, 'b) ne" is
-  "\<lambda>c x. lim (ne_chain c x)"
-  by (metis (no_types, lifting) Rep_ne core_compl mem_Collect_eq ne_chain.rep_eq non_expansive_def 
-    ofe_sym ofe_trans)
-instance apply standard apply (simp add: n_equiv_ne_def lim_ne.rep_eq ne_chain_def)
-  by (smt (verit, best) Abs_chain_inverse Rep_chain core_compl mem_Collect_eq ne_chain.rep_eq)
-end
-
-lift_definition ne_id :: "'a::ofe -n> 'a" is "id" by (rule non_expansiveI) simp
-lift_definition ne_const :: "'b::ofe \<Rightarrow> 'a::ofe -n> 'b" is "\<lambda>b _. b" 
-  by (rule non_expansiveI) (rule ofe_refl)
-
-lift_definition ne_comp :: "'b::ofe -n> 'c::ofe \<Rightarrow> 'a::ofe -n> 'b \<Rightarrow> 'a-n>'c" is
-  "\<lambda>f g. f \<circ> g" by (rule ne_comp)
-
-definition ne_map :: "('a2::ofe-n>'a1::ofe) \<Rightarrow> ('b1::ofe-n>'b2::ofe) \<Rightarrow> ('a1-n>'b1) \<Rightarrow> ('a2-n>'b2)" where
-  "ne_map f g h = ne_comp g (ne_comp h f)"
-
-lift_definition ne_map_ne :: "('a2::ofe-n>'a1::ofe) \<Rightarrow> ('b1::ofe-n>'b2::ofe) \<Rightarrow> (('a1-n>'b1)-n>('a2-n>'b2))" is
-  "\<lambda>f g. ne_map f g" unfolding ne_map_def ne_comp_def apply simp using ne_comp Rep_ne_inverse
-  by (smt (verit) Rep_ne mem_Collect_eq n_equiv_ne.rep_eq ne_comp.rep_eq non_expansive_def o_def)
-  
-subsection \<open>Contractive functions\<close>
-definition contractive :: "('a::ofe \<Rightarrow> 'b::ofe) \<Rightarrow> bool" where
-  "contractive con \<equiv> \<forall>n x y. (\<forall>m<n. n_equiv m x y) \<longrightarrow> n_equiv n (con x) (con y)"  
-
-definition contractive_alt :: "('a::ofe \<Rightarrow> 'b::ofe) \<Rightarrow> bool" where
-  "contractive_alt f \<equiv> \<forall>n x y. (case n of 0 \<Rightarrow> True | Suc n' \<Rightarrow> n_equiv n' x y) \<longrightarrow> n_equiv n (f x) (f y)"
-
-lemma contr_contr_alt: "contractive f \<longleftrightarrow> contractive_alt f"
-  apply (simp add: contractive_def contractive_alt_def split: nat.splits)
-  by (smt (verit, ccfv_SIG) bot_nat_0.extremum_strict ex_least_nat_less less_Suc_eq_le nat_less_le ofe_down_contr order.refl)
-
-lemma contractiveI: "(\<And>n x y. (\<forall>m<n. n_equiv m x y) \<Longrightarrow> n_equiv n (f x) (f y)) \<Longrightarrow> contractive f"
-  by (auto simp: contractive_def)
-
-lemma contractiveE: "contractive f \<Longrightarrow> (\<And>n x y. (\<forall>m<n. n_equiv m x y) \<Longrightarrow> n_equiv n (f x) (f y))"
-  by (auto simp: contractive_def)
-  
-lemma contractive_non_expansive: "contractive f \<Longrightarrow> non_expansive f"
-  by (auto simp: less_imp_le_nat intro: non_expansiveI ofe_mono[OF less_imp_le_nat] elim!: contractiveE)
-
-lemma next_contr: "contractive Next"
-  apply (rule contractiveI) 
-  apply (simp add: n_equiv_later_def)
-  using diff_Suc_less by blast
-  
-text \<open>The corresponding subtype of contractive functions.\<close>
-typedef (overloaded) ('a::ofe,'b::ofe) contr = "{f::'a\<Rightarrow>'b. contractive f}"
-  using contractiveI ofe_eq_limit by fastforce
-setup_lifting type_definition_contr
-lemmas [simp] = Rep_contr_inverse Rep_contr_inject
-lemmas [simp, intro!] = Rep_contr[unfolded mem_Collect_eq]
-
 subsection \<open>Resource Algebra\<close>
 class ra =
   fixes valid :: "'a \<Rightarrow> bool"
@@ -302,7 +186,7 @@ end
 lemma core_id: "core (a::'a::{core_id,total_camera}) = a"
   by (simp add: the_core_id core_def)
 
-text \<open>The semantics of the core_id class but for single values.\<close>
+text \<open>The semantics of the \<^class>\<open>core_id\<close> class but for single values.\<close>
 definition pcore_id_pred :: "'a::total_camera \<Rightarrow> bool" where
   "pcore_id_pred a \<equiv> pcore a = Some a"  
 
