IrisCore/iPropShallow.thy
@@ -1,9 +1,9 @@
-theory iPropShallow
-imports CoreStructures DerivedConstructions "../SpanningTree/SpanningTreeCameras" Namespace
-  BaseLogicShallow  
+theory iPropShallow                                                      
+imports DerivedConstructions "../SpanningTree/SpanningTreeCameras" Namespace
+  BaseLogicShallow "../HeapLang/PrimitiveLaws"
 begin
 
-text \<open>
+(*
   The functorial definition of iprop is as follows (unused arguments omitted):
 
   gampF := ((loc\<rightharpoonup>((loc option\<times>loc option) ex))\<times>frac) option auth
@@ -12,23 +12,19 @@ text \<open>
   heapF := (loc\<rightharpoonup>(dfrac\<times>val ag)) auth
   (b,_) resf := gmapF \<times> markingF \<times> b invF \<times> heapF
   iprop := (iprop,iprop) resf upred
-\<close>
+*)
 
 type_synonym 'a pre_inv = "(name\<rightharpoonup>'a later ag) auth \<times> name dset \<times> name dfset"
-type_synonym ('a,'b) resF = "graphUR auth \<times> markingUR auth \<times> 'a pre_inv \<times> heapGS"
+type_synonym ('a,'b) resF = "graphUR auth \<times> markingUR auth \<times> 'a pre_inv \<times> heap_lang_heap"
 
 text \<open> Axiomatic fixed point definition of iprop.\<close>
 typedecl pre_iprop
 instance pre_iprop :: ofe sorry
 type_synonym inv = "pre_iprop pre_inv"
 type_synonym res = "(pre_iprop,pre_iprop) resF"
-type_synonym res_pred = "res upred_f"
+type_synonym iprop = "res upred_f"
 
-typedef (overloaded) iprop = "UNIV::res_pred set" morphisms pred iProp ..
+axiomatization iProp :: "pre_iprop \<Rightarrow> iprop" and pre :: "iprop \<Rightarrow> pre_iprop"
+lemma iprop_fp: "iProp (pre P) = P" sorry
 declare [[coercion iProp]]
-
-setup_lifting type_definition_iprop
-
-lift_definition iPure :: "bool \<Rightarrow> iprop" ("\<upharpoonleft>_") is "upred_pure::bool \<Rightarrow> res_pred" .
-lift_definition iOwn :: "res \<Rightarrow> iprop" ("Own(_)") is "upred_own::res \<Rightarrow> res_pred" .
 end
