HeapLang/HeapLang.thy
@@ -6,7 +6,7 @@ begin
 
 section \<open> HeapLang Definition \<close>
 text \<open> The basic language definition \<close>
-text \<open> Based on https://gitlab.mpi-sws.org/iris/iris/-/blob/master/iris_heap_lang/lang.v\<close>
+text \<open> Based on \<^url>\<open>https://gitlab.mpi-sws.org/iris/iris/-/blob/master/iris_heap_lang/lang.v\<close> \<close>
 
 type_synonym proph_id = nat
 
