HeapLang/Spawn.thy
@@ -1,10 +1,10 @@
 theory Spawn
-imports HeapLang Notation "../IrisCore/DerivedConstructions"
+imports HeapLang Notation
 begin
 
 subsection \<open> Spawn and Join \<close>
 text \<open> More sophisticated concurrent primitives,
-  based on https://gitlab.mpi-sws.org/iris/iris/-/blob/master/iris_heap_lang/lib/spawn.v\<close>
+  based on \<^url>\<open>https://gitlab.mpi-sws.org/iris/iris/-/blob/master/iris_heap_lang/lib/spawn.v\<close>\<close>
 
 definition spawn :: val where "spawn \<equiv>
   V\<lambda> Some ''f'':
