IrisCore/BaseLogicDeep.thy
@@ -1,47 +1,8 @@
 theory BaseLogicDeep
-imports CoreStructures LogicSyntaxDeep
+imports CoreStructures LogicSyntaxDeep "../HeapLang/State" LogicTypesDeep
 begin
 
 section \<open> Base Logic \<close>
-text \<open> The axiomatized and simplified Iris base logic_term \<close>
-
-inductive well_typed :: "(string\<times>logic_type) list \<Rightarrow> 'a::ucamera logic_term \<Rightarrow> logic_type \<Rightarrow> bool" 
-  ("_\<turnstile>_:_" 60) where
-  ReflT: "[(x,\<tau>)] \<turnstile> Var x:\<tau>"
-| WeakenT: "\<Gamma>\<turnstile>t:\<tau> \<Longrightarrow> (x,\<tau>')#\<Gamma>\<turnstile>t:\<tau>"
-| SubstT: "(y,\<tau>')#(x,\<tau>')#\<Gamma>\<turnstile>t:\<tau> \<Longrightarrow> (x,\<tau>')#\<Gamma>\<turnstile>(var_subst (id(y:=x)) t):\<tau>"
-| SwitchT: "\<Gamma>2@(x,\<tau>1)#(y,\<tau>2)#\<Gamma>1\<turnstile>t:\<tau> \<Longrightarrow> \<Gamma>2@(x,\<tau>2)#(y,\<tau>1)#\<Gamma>1\<turnstile>(var_subst (id(y:=x,x:=y)) t):\<tau>"
-| UnitT: "\<Gamma>\<turnstile>Unit:UnitT"
-| ProdT: "\<lbrakk>\<Gamma>\<turnstile>t:\<tau>1;\<Gamma>\<turnstile>u:\<tau>2\<rbrakk> \<Longrightarrow> \<Gamma>\<turnstile>Prod(t,u):ProdT(\<tau>1,\<tau>2)"
-| FstT: "\<Gamma>\<turnstile>t:ProdT(\<tau>,\<tau>') \<Longrightarrow> \<Gamma>\<turnstile>Fst t:\<tau>"
-| SndT: "\<Gamma>\<turnstile>t:ProdT(\<tau>',\<tau>) \<Longrightarrow> \<Gamma>\<turnstile>Snd t:\<tau>"
-| LeftT: "\<Gamma>\<turnstile>t:\<tau> \<Longrightarrow> \<Gamma>\<turnstile>Left t:SumT \<tau> \<tau>'"
-| RightT: "\<Gamma>\<turnstile>t:\<tau> \<Longrightarrow> \<Gamma>\<turnstile>Right t:SumT \<tau>' \<tau>"
-| MatchT: "\<lbrakk>\<Gamma>\<turnstile>t:SumT \<tau>1 \<tau>2;(x,\<tau>1)#\<Gamma>\<turnstile>t1:\<tau>;(y,\<tau>2)#\<Gamma>\<turnstile>t2:\<tau>\<rbrakk> \<Longrightarrow> \<Gamma>\<turnstile>Match t x t1 y t2:\<tau>"
-| AbsT: "(x,\<tau>)#\<Gamma>\<turnstile>t:\<tau>' \<Longrightarrow> \<Gamma>\<turnstile>Abs x \<tau> t:FunT \<tau> \<tau>'"
-| AppT: "\<lbrakk>\<Gamma>\<turnstile>t:FunT \<tau> \<tau>';\<Gamma>\<turnstile>u:\<tau>\<rbrakk> \<Longrightarrow> \<Gamma>\<turnstile>App t u:\<tau>'"
-| ConstT: "\<Gamma>\<turnstile>Const a:M"
-| CoreT: "\<Gamma>\<turnstile>a:M \<Longrightarrow> \<Gamma>\<turnstile>Core a:M"
-| CompT: "\<lbrakk>\<Gamma>\<turnstile>a:M;\<Gamma>\<turnstile>b:M\<rbrakk> \<Longrightarrow> \<Gamma>\<turnstile>Comp a b:M"
-| FalseT: "\<Gamma>\<turnstile>FalseTrm:PropT"
-| TrueT: "\<Gamma>\<turnstile>TrueTrm:PropT"
-| EqT: "\<lbrakk>\<Gamma>\<turnstile>t:\<tau>;\<Gamma>\<turnstile>u:\<tau>\<rbrakk> \<Longrightarrow> \<Gamma>\<turnstile>EqTrm \<tau> t u:PropT"
-| ImplT: "\<lbrakk>\<Gamma>\<turnstile>P:PropT;\<Gamma>\<turnstile>Q:PropT\<rbrakk> \<Longrightarrow> \<Gamma>\<turnstile>Impl P Q:PropT"
-| ConjT: "\<lbrakk>\<Gamma>\<turnstile>P:PropT;\<Gamma>\<turnstile>Q:PropT\<rbrakk> \<Longrightarrow> \<Gamma>\<turnstile>Conj P Q:PropT"
-| DisjT: "\<lbrakk>\<Gamma>\<turnstile>P:PropT;\<Gamma>\<turnstile>Q:PropT\<rbrakk> \<Longrightarrow> \<Gamma>\<turnstile>Disj P Q:PropT"
-| SepT: "\<lbrakk>\<Gamma>\<turnstile>P:PropT;\<Gamma>\<turnstile>Q:PropT\<rbrakk> \<Longrightarrow> \<Gamma>\<turnstile>Sep P Q:PropT"
-| WandT: "\<lbrakk>\<Gamma>\<turnstile>P:PropT;\<Gamma>\<turnstile>Q:PropT\<rbrakk> \<Longrightarrow> \<Gamma>\<turnstile>Wand P Q:PropT"
-(* \<tau> also needs to be complete and inhabited but I have no idea how to formalize this. *)
-| GuardedT: "\<lbrakk>guarded x t;(x,\<tau>)#\<Gamma>\<turnstile>t:\<tau>\<rbrakk> \<Longrightarrow> \<Gamma>\<turnstile>Guarded x \<tau> t:\<tau>"
-| ExistsT: "(x,\<tau>)#\<Gamma>\<turnstile>P:PropT \<Longrightarrow> \<Gamma>\<turnstile>Exists x \<tau> P:PropT"
-| ForallT: "(x,\<tau>)#\<Gamma>\<turnstile>P:PropT \<Longrightarrow> \<Gamma>\<turnstile>Forall x \<tau> P:PropT"
-| OwnT: "\<Gamma>\<turnstile>a:M \<Longrightarrow> \<Gamma>\<turnstile>Own a:PropT"
-(* Due to this predicate being defined inside base_logic, M is a camera. *)
-| ValidT: "\<Gamma>\<turnstile>a:M \<Longrightarrow> \<Gamma>\<turnstile>Valid a:PropT"
-| PersistentT: "\<Gamma>\<turnstile>P:PropT \<Longrightarrow> \<Gamma>\<turnstile>Persistent P:PropT"
-| PlainT: "\<Gamma>\<turnstile>P:PropT \<Longrightarrow> \<Gamma>\<turnstile>Plain P:PropT"
-| LaterT: "\<Gamma>\<turnstile>P:PropT \<Longrightarrow> \<Gamma>\<turnstile>Later P:PropT"
-| UpdT: "\<Gamma>\<turnstile>P:PropT \<Longrightarrow> \<Gamma>\<turnstile>Upd P:PropT"
 
 (* Irrelevant contexts that were left out in the description are called I instead of \<Gamma>.  *)
 inductive judgement :: "(string\<times>logic_type) list \<Rightarrow> 'a::ucamera logic_term \<Rightarrow> 'a logic_term \<Rightarrow> bool" 
@@ -64,6 +25,14 @@ inductive judgement :: "(string\<times>logic_type) list \<Rightarrow> 'a::ucamer
 | ForallE: "\<lbrakk>\<Gamma>|P\<turnstile>Forall x \<tau> Q; \<Gamma>\<turnstile>t:\<tau>\<rbrakk> \<Longrightarrow> \<Gamma>|P\<turnstile>term_subst t x Q"
 | ExistsI: "\<lbrakk>\<Gamma>|P\<turnstile>term_subst t x Q; \<Gamma>\<turnstile>t:\<tau>\<rbrakk> \<Longrightarrow> \<Gamma>|P\<turnstile>Exists x \<tau> Q"
 | ExistsE: "(x,\<tau>)#\<Gamma>|P\<turnstile>Q \<Longrightarrow> \<Gamma>|Exists x \<tau> P\<turnstile>Q"
-| EtaRed: "I|P\<turnstile>Q \<Longrightarrow> I|P\<turnstile>Abs x \<tau> (App Q (Var x))"
+| EtaRed: "I|P\<turnstile>Q \<Longrightarrow> I|P\<turnstile>Abs x \<tau> (AppL Q (VarL x))"
 
+
+datatype 'a semantic_type = PropS "'a \<Rightarrow> nat \<Rightarrow> bool" | CmraS 'a | UnitS unit 
+  | SumS "'a semantic_type + 'a semantic_type" | ProdT "'a semantic_type\<times>'a semantic_type" 
+  | FunT "'a semantic_type fset"
+  | Expr expr | State state | Observation observation | List "'a semantic_type list"
+
+fun logic_semantic :: "'a::ucamera logic_term \<Rightarrow> 'a semantic_type" where
+  "logic_semantic Unit = UnitS ()"
 end
