IrisCore/BasicTypes.thy
@@ -1,0 +1,163 @@
+theory BasicTypes
+imports Main "HOL-Library.FSet"
+begin
+
+subsection \<open>Basic types of camera combinators\<close>
+
+subsubsection \<open>Disjoint set type\<close>
+text \<open> Set with extra bottom element to encode non-disjoint unions \<close>
+datatype 'a dset = DSet "'a set" | DBot
+
+subsubsection \<open>Disjoint finite set type\<close>
+text \<open> Finite set with extra bottom element to encode non-disjoint unions \<close>
+datatype 'a dfset = DFSet "'a fset" | DFBot
+
+subsubsection \<open>Extended sum type\<close>
+datatype ('a,'b) sum_ext = Inl 'a | Inr 'b | Inv
+
+type_notation sum_ext (infixl "+\<^sub>e" 15)
+lemmas sum_ex2 = sum_ext.exhaust[case_product sum_ext.exhaust]
+lemmas sum_ex3 = sum_ext.exhaust[case_product sum_ex2]
+lemmas sum_ex4 = sum_ext.exhaust[case_product sum_ex3]
+
+subsubsection \<open>Step indexed predicates\<close>
+text \<open>They are defined to hold for all steps below a maximum. \<close>
+typedef sprop = "{s::nat\<Rightarrow>bool. \<forall>n m. m\<le>n \<longrightarrow> s n \<longrightarrow> s m}"
+proof
+  define s :: "nat\<Rightarrow>bool" where "s = (\<lambda>_. True)"
+  thus "s \<in> {s::nat\<Rightarrow>bool. \<forall>n m. m\<le>n \<longrightarrow> s n \<longrightarrow> s m}" by simp
+qed
+
+setup_lifting type_definition_sprop
+lemmas [simp] = Rep_sprop_inverse Rep_sprop_inject
+lemmas [simp, intro!] = Rep_sprop[unfolded mem_Collect_eq]
+
+lift_definition sPure :: "bool \<Rightarrow> sprop" is "\<lambda>b _. b" .
+lemma sPureId: "Rep_sprop (Abs_sprop ((\<lambda>b _. b) b)) n = b"
+  using Abs_sprop_inverse by auto
+definition sFalse :: sprop where [simp]: "sFalse \<equiv> sPure False"
+definition sTrue :: sprop where [simp]: "sTrue \<equiv> sPure True"
+lemmas [simp] = sPure.rep_eq sPureId sPureId[simplified sPure.abs_eq[symmetric]]
+
+lift_definition n_subseteq :: "nat \<Rightarrow> sprop \<Rightarrow> sprop \<Rightarrow> bool" is
+  "\<lambda>n X Y. \<forall>m\<le>n. X m \<longrightarrow> Y m" .
+lift_definition sprop_conj :: "sprop \<Rightarrow> sprop \<Rightarrow> sprop" (infixl "\<and>\<^sub>s" 60) is 
+  "\<lambda>x y. (\<lambda>n. x n \<and> y n)" using conj_forward by simp
+lift_definition sprop_disj :: "sprop \<Rightarrow> sprop \<Rightarrow> sprop" (infixl "\<or>\<^sub>s" 60) is
+  "\<lambda>x y. (\<lambda>n. x n \<or> y n)" using disj_forward by simp
+lift_definition sprop_impl :: "sprop \<Rightarrow> sprop \<Rightarrow> sprop" (infixr "\<longrightarrow>\<^sub>s" 60) is
+  "\<lambda>x y. (\<lambda>n. \<forall>m\<le>n. x m \<longrightarrow> y m)" by (meson dual_order.trans)
+
+subsubsection \<open>Later camera combinator\<close>
+text \<open>This type encodes the later modality on a type level.\<close>
+datatype 'a later = Next (later_car: 'a)
+
+lemmas later2_ex = later.exhaust[case_product later.exhaust]
+lemmas later3_ex = later.exhaust[case_product later2_ex]
+
+subsubsection \<open>Agreement camera combinator\<close>
+typedef 'a ag = "{a::'a set | a. finite a \<and> a\<noteq>{} }"
+  by auto
+
+setup_lifting type_definition_ag
+
+lift_definition map_ag :: "('a\<Rightarrow>'b) \<Rightarrow> 'a ag \<Rightarrow> 'b ag" is "(`)" by simp
+lift_definition pred_ag :: "('a \<Rightarrow> bool) \<Rightarrow> 'a ag \<Rightarrow> bool" is "\<lambda>P s. Ball s P" .
+lift_definition rel_ag :: "('a \<Rightarrow> 'b \<Rightarrow> bool) \<Rightarrow> 'a ag \<Rightarrow> 'b ag \<Rightarrow> bool" is rel_set .
+
+lemma image_ag: "image f (Rep_ag s) \<in> {a |a. finite a \<and> a \<noteq> {}}"
+  apply (simp_all add: image_def)
+  apply (rule conjI)
+  subgoal using finite_imageI[unfolded image_def] Rep_ag by auto
+  using Rep_ag by fast
+lemmas image_abs_ag = Abs_ag_inverse[OF image_ag] Abs_ag_inject[OF image_ag  image_ag]
+
+context includes cardinal_syntax begin
+bnf "'a ag"
+  map: map_ag
+  sets: Rep_ag
+  bd: "natLeq"
+  rel: rel_ag
+proof -
+show "map_ag id = id" by (auto simp: map_ag_def Rep_ag_inverse)
+next
+fix f :: "'a \<Rightarrow> 'b" and g :: "'b \<Rightarrow> 'c"
+show "map_ag (g \<circ> f) = map_ag g \<circ> map_ag f" 
+  by (auto simp: comp_def image_def map_ag_def)
+  (metis Rep_ag_inverse image_def image_image map_ag.rep_eq map_fun_apply)
+next
+fix x :: "'a ag" and f g :: "'a \<Rightarrow> 'b"
+assume "\<And>z. z \<in> Rep_ag x \<Longrightarrow> f z = g z"
+then show "map_ag f x = map_ag g x" by transfer auto
+next
+fix f :: "'a\<Rightarrow>'b"
+have "{y. \<exists>x\<in>Rep_ag s. y = f x} = image f (Rep_ag s)" for s by auto
+then have "{y. \<exists>x\<in>Rep_ag s. y = f x} \<in> {a |a. finite a \<and> a \<noteq> {}}" for s
+  apply simp_all
+  apply (rule conjI)
+  subgoal using finite_imageI Rep_ag by fast
+  using Rep_ag by blast
+from Abs_ag_inverse[OF this] show "Rep_ag \<circ> map_ag f = (`) f \<circ> Rep_ag" 
+  by (auto simp: map_ag_def image_def comp_def)
+next
+show "card_order (natLeq )"
+  using card_of_card_order_on card_order_csum natLeq_card_order by blast
+next
+show "cinfinite (natLeq )"
+  using cinfinite_csum natLeq_cinfinite by blast
+next
+fix s :: "'a ag"
+show "|Rep_ag s| \<le>o natLeq"
+by (metis (no_types, lifting) Rep_ag card_of_Well_order infinite_iff_natLeq_ordLeq mem_Collect_eq 
+  natLeq_Well_order not_ordLeq_iff_ordLess ordLess_imp_ordLeq)
+next
+fix R :: "'a\<Rightarrow>'b\<Rightarrow>bool" and S :: "'b\<Rightarrow>'c\<Rightarrow>bool"
+show "rel_ag R OO rel_ag S \<le> rel_ag (R OO S)"
+  by (auto simp: rel_ag.rep_eq rel_set_def relcompp.simps) blast+
+next
+fix R :: "'a\<Rightarrow>'b\<Rightarrow>bool"
+show "rel_ag R = (\<lambda>x y. \<exists>z. Rep_ag z \<subseteq> {(x, y). R x y} \<and> map_ag fst z = x \<and> map_ag snd z = y)"
+apply (auto simp: rel_ag_def map_ag_def rel_set_def map_fun_def comp_def)
+apply standard
+apply standard
+proof
+  fix a :: "'a ag" and b :: "'b ag"
+  assume "(\<forall>x\<in>Rep_ag a. \<exists>xa\<in>Rep_ag b. R x xa) \<and> (\<forall>y\<in>Rep_ag b. \<exists>x\<in>Rep_ag a. R x y)"
+  then have assms: "\<forall>x\<in>Rep_ag a. \<exists>xa\<in>Rep_ag b. R x xa" "\<forall>y\<in>Rep_ag b. \<exists>x\<in>Rep_ag a. R x y" by simp_all
+  define c where c:"c = {(x,y) | x y. x\<in>Rep_ag a \<and> y\<in>Rep_ag b}"
+  from Rep_ag have "finite (Rep_ag a)" "Rep_ag a \<noteq> {}" "finite (Rep_ag b)" "Rep_ag b \<noteq> {}" by auto
+  with c have c_ag: "finite c" "c \<noteq> {}" by auto
+  define c' where c': "c' = c \<inter> {(x,y) | x y. R x y}"
+  with c_ag c and assms have c'_ag: "finite c'" "c' \<noteq> {}" by auto
+  from c' c assms have c'_alt: "c' = {(x,y) | x y. x\<in>Rep_ag a \<and> y\<in>Rep_ag b \<and> R x y}" by auto
+  define z where z: "z = Abs_ag c'"
+  then have rep_z: "Rep_ag z = c'" using Abs_ag_inverse c'_ag by auto
+  {
+    from c'_alt assms(1) have "(fst ` c') = Rep_ag a" by (simp add: image_def) blast
+    with rep_z have "Abs_ag (fst ` Rep_ag z) = a" using Rep_ag_inverse by auto
+  }
+  moreover {
+    from c'_alt assms(2) have "(snd ` c') = Rep_ag b" by (simp add: image_def) blast
+    with rep_z have "Abs_ag (snd ` Rep_ag z) = b" using Rep_ag_inverse by auto
+  }
+  moreover have "Rep_ag z \<subseteq> {(x, y). R x y}" using rep_z c' by simp
+  ultimately show "\<exists>z. Rep_ag z \<subseteq> {(x, y). R x y} \<and> Abs_ag (fst ` Rep_ag z) = a \<and> Abs_ag (snd ` Rep_ag z) = b"
+  by auto
+next
+  fix a :: "'a ag" and b :: "'b ag"
+  assume "\<exists>z. Rep_ag z \<subseteq> {(x, y). R x y} \<and> Abs_ag (fst ` Rep_ag z) = a \<and> Abs_ag (snd ` Rep_ag z) = b"
+  then show "(\<forall>x\<in>Rep_ag a. \<exists>xa\<in>Rep_ag b. R x xa) \<and> (\<forall>y\<in>Rep_ag b. \<exists>x\<in>Rep_ag a. R x y)"
+  by (smt (verit, best) Product_Type.Collect_case_prodD image_abs_ag(1) image_iff subset_eq)
+qed
+qed
+end
+
+subsubsection \<open>Exclusive camera combinator\<close>
+datatype 'a ex = Ex 'a | Inv
+
+subsubsection \<open>Authoritative camera combinator\<close>
+datatype 'm auth = Auth "('m ex option\<times>'m)"
+
+abbreviation fragm :: "'m \<Rightarrow> 'm auth" where "fragm \<equiv> \<lambda>a::'m. Auth (None, a)"
+abbreviation comb :: "'m \<Rightarrow> 'm \<Rightarrow> 'm auth" where "comb \<equiv> \<lambda>(a::'m) b. Auth (Some (Ex a), b)"
+end
