IrisCore/COFEs.thy
@@ -1,0 +1,96 @@
+theory COFEs
+imports NonExpansive
+begin
+
+subsection \<open> COFE \<close>
+typedef (overloaded) 't chain = "{c::(nat \<Rightarrow> 't::ofe). \<forall>n m. n\<le>m \<longrightarrow> n_equiv n (c m) (c n)}"
+  using ofe_eq_limit by force
+setup_lifting type_definition_chain
+lemmas [simp] = Rep_chain_inverse Rep_chain_inject
+lemmas [simp, intro!] = Rep_chain[unfolded mem_Collect_eq]
+
+class cofe = ofe +
+  fixes lim :: "('a::ofe) chain \<Rightarrow> 'a"
+  assumes core_compl: "n_equiv n (lim c) (Rep_chain c n)"
+
+instantiation unit :: cofe begin
+definition lim_unit :: "unit chain \<Rightarrow> unit" where [simp]: "lim_unit _ = ()"
+instance by standard (simp add: n_equiv_unit_def)
+end
+
+lift_definition option_chain :: "'a::ofe option chain \<Rightarrow> 'a \<Rightarrow> 'a chain" is
+  "\<lambda>c x n. case c n of Some y \<Rightarrow> y | None \<Rightarrow> x" 
+  by (auto simp: ofe_refl n_equiv_option_def split: option.splits) fastforce+
+
+instantiation option :: (cofe) cofe begin
+definition lim_option :: "'a option chain \<Rightarrow> 'a option" where
+  "lim_option c \<equiv> case (Rep_chain c 0) of Some x \<Rightarrow> Some (lim (option_chain c x)) | None \<Rightarrow> None"
+instance proof
+  fix c :: "'a option chain" and n
+  have base: "n_equiv 0 (Rep_chain c n) (Rep_chain c 0)" by transfer auto
+  from core_compl have step: "n_equiv n (lim (option_chain c x)) (Rep_chain (option_chain c x) n)" for x .
+  show "n_equiv n (lim c) (Rep_chain c n)" unfolding lim_option_def
+  apply (cases "Rep_chain c 0")
+  apply simp_all
+  apply (metis base n_equiv_option_def option.distinct(1))
+  by (smt (verit) base step n_equiv_option_def option.simps(5) option_chain.rep_eq)
+qed
+end
+
+lift_definition later_chain :: "'a::ofe later chain \<Rightarrow> 'a chain" is
+  "\<lambda>c n. later_car (Rep_chain c (Suc n))" 
+  by transfer (metis Suc_le_mono add_diff_cancel_left' n_equiv_later_def nat.discI plus_1_eq_Suc)
+
+instantiation later :: (cofe) cofe begin
+definition lim_later :: "'a later chain \<Rightarrow> 'a later" where
+  "lim_later c = Next (lim (later_chain c))"
+instance proof
+  fix c :: "'a later chain" and n
+  from core_compl[of n] show "n_equiv n (lim c) (Rep_chain c n)" 
+    apply (simp add: n_equiv_later_def lim_later_def)
+    by (smt (verit, ccfv_threshold) Suc_pred bot_nat_0.not_eq_extremum core_compl later_chain.rep_eq)
+qed
+end
+
+definition discrete_lim :: "('a::discrete chain) \<Rightarrow> 'a" where
+  "discrete_lim c = Rep_chain c 0"
+
+lemma discrete_cofe: "n_equiv n (discrete_lim c) (Rep_chain c n)"
+  unfolding discrete_lim_def by transfer (metis d_equiv nat_le_linear)
+
+subsection \<open>COFE instances\<close>
+subsubsection \<open>Product type COFE\<close>
+lift_definition chain_map :: "('a::ofe -n> 'b::ofe) \<Rightarrow> 'a chain \<Rightarrow> 'b chain" is
+  "\<lambda>f c n. f (Rep_chain c n)" by transfer (simp add: non_expansive_def)
+
+lift_definition ne_fst :: "('a::ofe\<times>'b::ofe)-n>'a" is "\<lambda>(a,_). a" by (rule non_expansiveI) auto
+lift_definition ne_snd :: "('a::ofe\<times>'b::ofe)-n>'b" is "\<lambda>(_,b). b" by (rule non_expansiveI) auto
+
+instantiation prod :: (cofe,cofe) cofe begin
+definition lim_prod :: "('a \<times> 'b) chain \<Rightarrow> 'a \<times> 'b" where 
+  "lim_prod c = (lim (chain_map ne_fst c), lim (chain_map ne_snd c))"
+instance proof 
+  fix c :: "('a\<times>'b) chain" and n
+  have "n_equiv n (lim (chain_map ne_fst c)) (Rep_chain (chain_map ne_fst c) n)" 
+    "n_equiv n (lim (chain_map ne_snd c)) (Rep_chain (chain_map ne_snd c) n)" 
+    using core_compl by auto  
+  then show "n_equiv n (lim c) (Rep_chain c n)"
+  apply (simp add: lim_prod_def ne_fst.rep_eq ne_snd.rep_eq chain_map_def)
+  by (smt (z3) Abs_chain_inverse Rep_chain case_prod_conv mem_Collect_eq n_equiv_prod.elims(2) n_equiv_prod.elims(3))
+qed
+end
+
+subsubsection \<open>Non expansive function COFE\<close>
+lift_definition ne_chain :: "('a::ofe,'b::ofe) ne chain \<Rightarrow> 'a \<Rightarrow> 'b chain" is
+  "\<lambda>c x n. Rep_ne (c n) x" apply transfer unfolding non_expansive_def by auto
+  
+instantiation ne :: (ofe,cofe) cofe begin
+lift_definition lim_ne :: "('a, 'b) ne chain \<Rightarrow> ('a, 'b) ne" is
+  "\<lambda>c x. lim (ne_chain c x)"
+  by (metis (no_types, lifting) Rep_ne core_compl mem_Collect_eq ne_chain.rep_eq non_expansive_def 
+    ofe_sym ofe_trans)
+instance apply standard apply (simp add: n_equiv_ne_def lim_ne.rep_eq ne_chain_def)
+  by (smt (verit, best) Abs_chain_inverse Rep_chain core_compl mem_Collect_eq ne_chain.rep_eq)
+end
+
+end
