IrisCore/Invariant.thy
@@ -14,7 +14,7 @@ begin
 
 text \<open>Allocate new invariant map\<close>
 definition ownI :: "name \<Rightarrow> iprop \<Rightarrow> iprop" where
-  "ownI \<iota> P = Own\<^sub>i (fragm [\<iota>\<mapsto>to_ag (Next P)],\<epsilon>,\<epsilon>)"
+  "ownI \<iota> P = Own\<^sub>i (fragm [\<iota>\<mapsto>to_ag (Next (pre P))],\<epsilon>,\<epsilon>)"
 
 definition inv :: "namespace \<Rightarrow> iprop \<Rightarrow>  iprop" where
   "inv N P = \<exists>\<^sub>u \<iota>. ((\<upharpoonleft>(\<iota>\<in>names N)) \<and>\<^sub>u ownI \<iota> P)"
@@ -27,26 +27,15 @@ text \<open>Allocate new disabled invariant map\<close>
 definition ownD :: "name dfset \<Rightarrow> iprop" where
   "ownD D = Own\<^sub>i (\<epsilon>,\<epsilon>,D)"  
   
-definition lift_inv_map :: "(name\<rightharpoonup>iprop) \<Rightarrow> (name\<rightharpoonup> iprop later ag)" where
-  "lift_inv_map = (\<circ>) (map_option (to_ag \<circ> Next))"
+definition lift_inv_map :: "(name\<rightharpoonup>iprop) \<Rightarrow> (name\<rightharpoonup> pre_iprop later ag)" where
+  "lift_inv_map = (\<circ>) (map_option (to_ag \<circ> Next \<circ> pre))"
   
 text \<open>World satisfaction, i.e. the invariant that holds all invariants\<close>
-(* Doesn't type check *)  
 definition wsat :: iprop where
   "wsat \<equiv> \<exists>\<^sub>u (I::name\<rightharpoonup>iprop).
     ((Own\<^sub>i(full(lift_inv_map I),\<epsilon>,\<epsilon>))
     \<^emph> (sep_map_set (\<lambda>\<iota>. ((\<triangleright>((the \<circ> I) \<iota>)) \<^emph> ownD (DFSet {|\<iota>|})) \<or>\<^sub>u (ownE (DSet {\<iota>}))) (dom I))
   )"
-\<comment> \<open> The problem here:
-  - Own\<^sub>i(full(lift_inv_map I),\<epsilon>,\<epsilon>) is of type  iprop, i.e. an iprop which 
-    talks about has resources in the heap ('l\<rightharpoonup>'v), in invariants (based on 'a) and the camera 'c
-
-  - \<triangleright>((the \<circ> I) \<iota> is of type 'a iprop, i.e. only talks about resources of camera 'a
-
-  - 'a would need to be the same as , which is a cyclic type definition and only
-    possible if we find a fixed point type
-\<close>
-  
 end
 
 lemma persistent_ownI: "persistent (ownI \<iota> P)"
