IrisCore/LogicTypesDeep.thy
@@ -1,0 +1,85 @@
+theory LogicTypesDeep
+imports LogicSyntaxDeep
+begin
+
+inductive well_typed :: "(string\<times>logic_type) list \<Rightarrow> 'a::ucamera logic_term \<Rightarrow> logic_type \<Rightarrow> bool" 
+  ("_\<turnstile>_:_" 60) where
+  ReflT: "[(x,\<tau>)] \<turnstile> VarL x:\<tau>"
+| WeakenT: "\<Gamma>\<turnstile>t:\<tau> \<Longrightarrow> (x,\<tau>')#\<Gamma>\<turnstile>t:\<tau>"
+| SubstT: "(y,\<tau>')#(x,\<tau>')#\<Gamma>\<turnstile>t:\<tau> \<Longrightarrow> (x,\<tau>')#\<Gamma>\<turnstile>(var_subst (id(y:=x)) t):\<tau>"
+| SwitchT: "\<Gamma>2@(x,\<tau>1)#(y,\<tau>2)#\<Gamma>1\<turnstile>t:\<tau> \<Longrightarrow> \<Gamma>2@(x,\<tau>2)#(y,\<tau>1)#\<Gamma>1\<turnstile>(var_subst (id(y:=x,x:=y)) t):\<tau>"
+| UnitT: "\<Gamma>\<turnstile>Unit:UnitT"
+| ProdT: "\<lbrakk>\<Gamma>\<turnstile>t:\<tau>1;\<Gamma>\<turnstile>u:\<tau>2\<rbrakk> \<Longrightarrow> \<Gamma>\<turnstile>Prod t u:ProdT \<tau>1 \<tau>2"
+| FstT: "\<Gamma>\<turnstile>t:ProdT \<tau> \<tau>' \<Longrightarrow> \<Gamma>\<turnstile>FstL t:\<tau>"
+| SndT: "\<Gamma>\<turnstile>t:ProdT \<tau>' \<tau> \<Longrightarrow> \<Gamma>\<turnstile>SndL t:\<tau>"
+| AbsT: "(x,\<tau>)#\<Gamma>\<turnstile>t:\<tau>' \<Longrightarrow> \<Gamma>\<turnstile>Abs x \<tau> t:FunT \<tau> \<tau>'"
+| AppT: "\<lbrakk>\<Gamma>\<turnstile>t:FunT \<tau> \<tau>';\<Gamma>\<turnstile>u:\<tau>\<rbrakk> \<Longrightarrow> \<Gamma>\<turnstile>AppL t u:\<tau>'"
+| ConstT: "\<Gamma>\<turnstile>Const a:CmraT"
+| CoreT: "\<Gamma>\<turnstile>a:CmraT \<Longrightarrow> \<Gamma>\<turnstile>Core a:CmraT"
+| CompT: "\<lbrakk>\<Gamma>\<turnstile>a:CmraT;\<Gamma>\<turnstile>b:CmraT\<rbrakk> \<Longrightarrow> \<Gamma>\<turnstile>Comp a b:CmraT"
+| FalseT: "\<Gamma>\<turnstile>FalseTrm:PropT"
+| TrueT: "\<Gamma>\<turnstile>TrueTrm:PropT"
+| EqT: "\<lbrakk>\<Gamma>\<turnstile>t:\<tau>;\<Gamma>\<turnstile>u:\<tau>\<rbrakk> \<Longrightarrow> \<Gamma>\<turnstile>EqTrm \<tau> t u:PropT"
+| ImplT: "\<lbrakk>\<Gamma>\<turnstile>P:PropT;\<Gamma>\<turnstile>Q:PropT\<rbrakk> \<Longrightarrow> \<Gamma>\<turnstile>Impl P Q:PropT"
+| ConjT: "\<lbrakk>\<Gamma>\<turnstile>P:PropT;\<Gamma>\<turnstile>Q:PropT\<rbrakk> \<Longrightarrow> \<Gamma>\<turnstile>Conj P Q:PropT"
+| DisjT: "\<lbrakk>\<Gamma>\<turnstile>P:PropT;\<Gamma>\<turnstile>Q:PropT\<rbrakk> \<Longrightarrow> \<Gamma>\<turnstile>Disj P Q:PropT"
+| SepT: "\<lbrakk>\<Gamma>\<turnstile>P:PropT;\<Gamma>\<turnstile>Q:PropT\<rbrakk> \<Longrightarrow> \<Gamma>\<turnstile>Sep P Q:PropT"
+| WandT: "\<lbrakk>\<Gamma>\<turnstile>P:PropT;\<Gamma>\<turnstile>Q:PropT\<rbrakk> \<Longrightarrow> \<Gamma>\<turnstile>Wand P Q:PropT"
+(* \<tau> also needs to be complete and inhabited but I have no idea how to formalize this. *)
+| GuardedT: "\<lbrakk>guarded x t;(x,\<tau>)#\<Gamma>\<turnstile>t:\<tau>\<rbrakk> \<Longrightarrow> \<Gamma>\<turnstile>Guarded x \<tau> t:\<tau>"
+| ExistsT: "(x,\<tau>)#\<Gamma>\<turnstile>P:PropT \<Longrightarrow> \<Gamma>\<turnstile>Exists x \<tau> P:PropT"
+| ForallT: "(x,\<tau>)#\<Gamma>\<turnstile>P:PropT \<Longrightarrow> \<Gamma>\<turnstile>Forall x \<tau> P:PropT"
+| OwnT: "\<Gamma>\<turnstile>a:CmraT \<Longrightarrow> \<Gamma>\<turnstile>Own a:PropT"
+| ValidT: "\<Gamma>\<turnstile>a:CmraT \<Longrightarrow> \<Gamma>\<turnstile>Valid a:PropT"
+| PersistentT: "\<Gamma>\<turnstile>P:PropT \<Longrightarrow> \<Gamma>\<turnstile>Persistent P:PropT"
+| PlainT: "\<Gamma>\<turnstile>P:PropT \<Longrightarrow> \<Gamma>\<turnstile>Plain P:PropT"
+| LaterT: "\<Gamma>\<turnstile>P:PropT \<Longrightarrow> \<Gamma>\<turnstile>Later P:PropT"
+| UpdT: "\<Gamma>\<turnstile>P:PropT \<Longrightarrow> \<Gamma>\<turnstile>Upd P:PropT"
+
+fun comb_option :: "'a option \<Rightarrow> 'a option \<Rightarrow> ('a \<Rightarrow> 'a \<Rightarrow> 'b) \<Rightarrow> 'b option" where
+  "comb_option (Some x) (Some y) f = Some (f x y)"
+| "comb_option _ _ _ = None"
+
+fun comb_option_eq :: "'a \<Rightarrow> 'a option \<Rightarrow> 'b \<Rightarrow> 'b option" where
+  "comb_option_eq e (Some x) C = (if x=e then Some C else None)"
+| "comb_option_eq _ _ _ = None"
+
+fun comb_option_eq2 :: "'a \<Rightarrow>'a option \<Rightarrow> 'a option \<Rightarrow> 'b \<Rightarrow> 'b option" where
+  "comb_option_eq2 e (Some x) (Some y) C = (if x=e\<and> y=e then Some C else None)"
+| "comb_option_eq2 _ _ _ _ = None"
+
+fun type_of_term :: "'a::ucamera logic_term \<Rightarrow> (string\<rightharpoonup>logic_type) \<Rightarrow> logic_type option" where
+  "type_of_term Unit _ = Some UnitT"
+| "type_of_term (VarL s) \<Gamma> = \<Gamma> s"
+| "type_of_term (Prod f s) \<Gamma> = comb_option (type_of_term f \<Gamma>) (type_of_term s \<Gamma>) ProdT"
+| "type_of_term (FstL p) \<Gamma> = 
+  (case type_of_term p \<Gamma> of Some (ProdT fT _) \<Rightarrow> Some fT | _ \<Rightarrow> None)"
+| "type_of_term (SndL p) \<Gamma> =
+  (case type_of_term p \<Gamma> of Some (ProdT _ sT) \<Rightarrow> Some sT | _ \<Rightarrow> None)"
+| "type_of_term (Abs v vT b) \<Gamma> = map_option (\<lambda>bT. FunT vT bT) (type_of_term b (\<Gamma>(v \<mapsto> vT)))"
+| "type_of_term (AppL f x) \<Gamma> = comb_option (type_of_term f \<Gamma>) (type_of_term x \<Gamma>) FunT"
+| "type_of_term (Const _) _ = Some CmraT"
+| "type_of_term (Core x) \<Gamma> = (case type_of_term x \<Gamma> of Some CmraT \<Rightarrow> Some CmraT | _ \<Rightarrow> None)"
+| "type_of_term (Comp x y) \<Gamma> = comb_option_eq2 CmraT (type_of_term x \<Gamma>) (type_of_term y \<Gamma>) CmraT"
+| "type_of_term FalseTrm _ = Some PropT"
+| "type_of_term TrueTrm _ = Some PropT"
+| "type_of_term (EqTrm \<tau> x y) \<Gamma> = comb_option_eq2 \<tau> (type_of_term x \<Gamma>) (type_of_term y \<Gamma>) PropT"
+| "type_of_term (Impl P Q) \<Gamma> = comb_option_eq2 PropT (type_of_term P \<Gamma>) (type_of_term Q \<Gamma>) PropT"
+| "type_of_term (Conj P Q) \<Gamma> = comb_option_eq2 PropT (type_of_term P \<Gamma>) (type_of_term Q \<Gamma>) PropT"
+| "type_of_term (Disj P Q) \<Gamma> = comb_option_eq2 PropT (type_of_term P \<Gamma>) (type_of_term Q \<Gamma>) PropT"
+| "type_of_term (Sep P Q) \<Gamma> = comb_option_eq2 PropT (type_of_term P \<Gamma>) (type_of_term Q \<Gamma>) PropT"
+| "type_of_term (Wand P Q) \<Gamma> = comb_option_eq2 PropT (type_of_term P \<Gamma>) (type_of_term Q \<Gamma>) PropT"
+| "type_of_term (Guarded v vT b) \<Gamma> = (if guarded v b then 
+  Option.bind (type_of_term b (\<Gamma>(v\<mapsto>vT))) (\<lambda>bT. if bT=vT then Some vT else None) else None)"
+| "type_of_term (Exists v vT b) \<Gamma> = Option.bind (type_of_term b (\<Gamma>(v\<mapsto>vT))) (\<lambda>_. Some PropT)"
+| "type_of_term (Forall v vT b) \<Gamma> = Option.bind (type_of_term b (\<Gamma>(v\<mapsto>vT))) (\<lambda>_. Some PropT)"
+| "type_of_term (Own x) \<Gamma> = comb_option_eq CmraT (type_of_term x \<Gamma>) PropT"
+| "type_of_term (Valid x) \<Gamma> = comb_option_eq CmraT (type_of_term x \<Gamma>) PropT"
+| "type_of_term (Persistent x) \<Gamma> = comb_option_eq PropT (type_of_term x \<Gamma>) PropT"
+| "type_of_term (Plain x) \<Gamma> = comb_option_eq PropT (type_of_term x \<Gamma>) PropT"
+| "type_of_term (Later x) \<Gamma> = comb_option_eq PropT (type_of_term x \<Gamma>) PropT"
+| "type_of_term (Upd x) \<Gamma> = comb_option_eq PropT (type_of_term x \<Gamma>) PropT"
+
+lemma "(type_of_term t (map_of \<Gamma>) = Some \<tau>) \<longleftrightarrow> \<Gamma>\<turnstile>t:\<tau>"
+sorry
+end
