IrisCore/iProp.thy
@@ -1,9 +1,0 @@
-theory iProp
-imports DerivedConstructions BaseLogicShallowAlt Frac AuthHeap Misc "../SpanningTree/SpanningTreeCameras"
-  Namespace 
-begin
-
-datatype invGS = Inv "(name\<rightharpoonup>iprop later ag) auth"
-  and iprop = iProp "invGS upred"
-
-end
