SpanningTree/SpanningTreeCameras.thy
@@ -2,7 +2,6 @@ theory SpanningTreeCameras
 imports Graph
   "../IrisCore/Frac"
   "../HeapLang/HeapLang"
-  "../HeapLang/PrimitiveLaws"
 begin
 
 (* Children locations, in Coq it's a leibniz0 structure*)
@@ -15,20 +14,4 @@ type_synonym graphUR = "((loc\<rightharpoonup>(chl ex))\<times>frac) option"
 type_synonym markingUR = "loc set"
 
 type_synonym spanningG = "(graphUR auth \<times> markingUR auth)"
-
-(* 
-  This would normally be a list of camera functors to allow for modular reasoning.
-  Isabelle does not support type lists and thus we use a tuple for this simple example.  
-
-type_synonym graphG = "(graphUR auth \<times> markingUR auth) heapGCmra"
-
-abbreviation own_graph :: "graphUR auth \<Rightarrow> graphG iprop" ("Own\<^sub>g _") where
-  "own_graph \<equiv> \<lambda>g. own_other(g, \<epsilon>)"
-abbreviation own_marking :: "markingUR auth \<Rightarrow> graphG iprop" ("Own\<^sub>m _") where
-  "own_marking \<equiv> \<lambda>m. own_other(\<epsilon>, m)"
-
-
-context includes points_to_syntax begin
-lemma  "upred_holds (((l \<mapsto>{dq} v)::graphG iprop) -\<^emph> \<upharpoonleft>(valid dq))" by (rule points_to_valid)
-end*)
 end
